
Tính (a / b) % m

## Định lí fermat nhỏ

Nếu **m** là số nguyên tố và **a** không chia hết cho **m** thì:

a<sup>m-1</sup> % m = 1

--------------
1 / b = b<sup>-1</sup>

a / b = a * b<sup>-1</sup>

(a / b) % m 
= (a * b<sup>-1</sup>) % m
= (a % m) * (b<sup>-1</sup> % m) % m


Đinh lí fermat nhỏ: b<sup>m-1</sup> % m = 1 % m

**b<sup>m-1</sup> % m = 1 % m**

Nhân cả 2 vế với b<sup>-1</sup>

b<sup>m-2</sup> % m = b<sup>-1</sup> % m

=> (a / b) % m = (a % m) * (b<sup>m-2</sup> % m) % m

Tổng quan.

(1 / b) % m = b<sup>-1</sup> % m
b<sup>-1</sup> = b<sup>m-2</sup> % m